Working on proofs in Left and Right Shift Nodes

Optimizations/Canonicalizations/LeftShiftPhase.thy
@@ -3,52 +3,106 @@ subsection \<open>LeftShiftNode Phase\<close>
 theory LeftShiftPhase
   imports
     Common
+    Proofs.StampEvalThms
 begin
 
 phase LeftShiftNode
   terminating size
 begin
 
+
 (*
-
-fun shift_amount :: "iwidth \<Rightarrow> int64 \<Rightarrow> nat" where
-  "shift_amount b val = unat (and val (if b = 64 then 0x3F else 0x1f))"
-
+fun shift_amount_new :: "iwidth \<Rightarrow> int64 \<Rightarrow> int64" where
+  "shift_amount_new b val = unat (and val (if b = 64 then 0x3F else 0x1f))"
 *)
 
 (* Value level proofs *)
-
-(* Need to transform to 32-bit only *)
-lemma val_EliminateRHS:
-  assumes "(val[y & (new_int 32 (31))] = new_int 32 0)"
+(* 64-bit version *)
+lemma val_EliminateRHS_64:
+  assumes "x = IntVal 64 vx"
+  and     "y = IntVal 64 vy"
+  and     "and vy (mask 6) = 0"
   and     "val[x << y] \<noteq> UndefVal"
-shows   "val[x << y] = x"
-  using assms apply (cases x; cases y; auto)
-  subgoal premises p for x22 x21a x22a
-  proof -
-      have "val_to_bool(val[(IntVal 32 31 < y)])"
-       using assms  sorry
-     then have "take_bit LENGTH(64) ((x22 << unat (and x22a (63))) :: 64 word) = x22"
-       unfolding Word.take_bit_length_eq 
- (* Values.shift_amount.simps *) (*Values.shiftl_def*)
-        sorry
-    then show ?thesis
-        by simp
-    qed
-
-  subgoal premises p for x21 x22 x21a x22a
+  shows "val[x << y] = x"
+  using assms apply (cases x; cases y; auto) 
+  subgoal
     proof -
-      have "take_bit x21 (x22 << unat (and x22a (31::64 word))) = x22"
-        sorry
+      have 1: "(and vy (63) = 0)"
+        using assms 
+        by (metis (no_types, lifting) Suc_1 add_2_eq_Suc' add_Suc_shift mask_1 mask_Suc_rec mult_2 
+            numeral_Bit0 numeral_Bit1 numeral_One)
+      then have 2: "(0::nat) mod (2::nat) ^ LENGTH(64) = 0"
+        by simp
+      then have 3: "(vx << 0) = vx"
+        unfolding shiftl_def
+        by simp
+      then have "take_bit LENGTH(64) ((vx << unat (and vy (63)))::64 word) = vx"
+        unfolding Word.take_bit_length_eq 1 Word.unat_word_ariths(4) 2 3 by auto
       then show ?thesis
-        sorry
+        by simp    
+     qed
+     done
+
+lemma val_EliminateRHS_642:
+  assumes "x = IntVal 64 vx"
+  and     "y = IntVal 64 vy"
+  and     "(shift_amount 64 vy) = 0"
+  and     "val[x << y] \<noteq> UndefVal"
+  shows "val[x << y] = x"
+  using assms apply (cases x; cases y; auto) 
+  subgoal
+    proof -
+       have 3: "(vx << 0) = vx"
+        unfolding shiftl_def
+        by simp
+      then have "take_bit LENGTH(64) ((vx << 0)::64 word) = vx"
+        unfolding Word.take_bit_length_eq by auto
+      then show ?thesis
+        by simp    
+     qed
+     done
+
+
+(* All bit-widths *)
+lemma val_EliminateRHS:
+  assumes "x = IntVal bx vx"
+  and     "bx = 32 | bx = 64"
+  and     "y = IntVal by vy"
+  and     "(shift_amount bx vy) = 0"
+  and     "val[x << y] \<noteq> UndefVal"
+  shows "val[x << y] = x"
+  using assms apply (cases x; cases y; auto)
+  subgoal (* 32-bit *)
+  proof -
+    have 1: "vx << (0::nat) = vx"
+      unfolding shiftl_def by simp
+    then have "take_bit 32 (vx << (0::nat)) = vx"
+      unfolding Word.take_bit_length_eq 1 
+      apply (cases vx; simp) 
+      
+      sorry
+      then show ?thesis
+        by simp    
     qed
-  done
+    subgoal (* 64-bit *)
+    proof -
+       have 3: "(vx << 0) = vx"
+        unfolding shiftl_def
+        by simp
+      then have "take_bit LENGTH(64) ((vx << 0)::64 word) = vx"
+        unfolding Word.take_bit_length_eq by auto
+      then show ?thesis
+        by simp    
+     qed
+   done
 
 (* Exp level proofs *)
 lemma exp_EliminateRHS:
-  assumes "val[y & (new_int 32 (31))] = new_int 32 0"
-  shows   "exp[x << const(y)] \<ge> x"
+  assumes "y = IntVal 64 vy"
+  and     "and vy (mask 6) = 0" 
+  and     "stamp_expr x = IntegerStamp 64 lo hi" 
+  and     "wf_stamp x"
+  shows "exp[x << const(y)] \<ge> x"
   unfolding bin_eval.simps(8) apply auto
   subgoal premises p for m p xa
     proof -
@@ -59,17 +113,19 @@ lemma exp_EliminateRHS:
       then have 2: "val[xa << y] \<noteq> UndefVal"
         using evalDet p(1) p(2) xa by blast
       then have "val[xa << y] = xa" 
-        using assms val_EliminateRHS by auto  
+        using assms val_EliminateRHS  sorry
       then show ?thesis
         using evalDet p(1) xa by fastforce
     qed
   done
 
 text \<open>Optimisations\<close>
-(* Need to prove val_EliminateRHS*)
-optimization EliminateRHS: "(x << const(y)) \<longmapsto> x when 
-                            (val[y & (new_int 32 (31))] = new_int 32 0)"
-  using exp_EliminateRHS  by auto
+
+
+optimization EliminateRHS_64: "(x << const(y)) \<longmapsto> x when 
+                               (stamp_expr x = IntegerStamp 64 lo hi \<and> 
+                                wf_stamp x)"
+  using exp_EliminateRHS wf_stamp_def  bin_eval.simps(8) sorry
 
 end (* End of ShiftNode *)
 
