Optimizations/Canonicalizations/RightShiftPhase.thy
@@ -1,0 +1,37 @@
+subsection \<open>RightShiftNode Phase\<close>
+
+theory RightShiftPhase
+  imports
+    Common
+    Proofs.StampEvalThms
+begin
+
+phase RightShiftNode
+  terminating size
+begin
+
+(* Value level proofs *)
+(* Has counter-example if x not 32-bit *)
+lemma val_ReturnXOnZeroShift:
+  assumes "val[x >> (IntVal 32 0)] \<noteq> UndefVal"
+  and     "x = IntVal 32 xv"
+  shows "val[x >> (IntVal 32 0)] = val[x]"  
+  using assms apply (cases x; auto)
+  sorry
+
+(* Exp level proofs *)
+lemma exp_ReturnXOnZeroShift:
+  assumes "stamp_expr x = IntegerStamp 32 lo hi"
+  and     "wf_stamp x"
+  shows "exp[x >> const(IntVal 32 0)] \<ge> exp[x]" 
+   sorry
+
+text \<open>Optimisations\<close>
+(* Need to prove exp_ReturnXOnZeroShift *)
+optimization ReturnXOnZeroShift: "(x >> const(new_int 32 0)) \<longmapsto> x when 
+                                  ((stamp_expr x = IntegerStamp 32 lo hi) \<and> (wf_stamp x))"
+   using exp_ReturnXOnZeroShift by fastforce
+
+end (* End of RightShiftNode *)
+
+end (* End of file *)
